\section*{Exercise 1}
A $2m$-order local interpolating polynomial to $u(x)$ in the neighborhood of $x_j$ given as
\begin{equation}
	u(x) = \sum_{k=-m}^m u_{j+k} L_{j+k}(x)
	\label{eq:interp_poly}
\end{equation}
where the grid function $u_{j+k} = u(x_{j+k})$ and the \textit{Lagrange interpolation polynomial} is
\begin{equation}
	L_{j+k} = \prod_{l=-m, l \neq k}^m \frac{x - x_{j+l}}{x_{j+k} - x_{j+l}}.
	\label{eq:lagrange_interpoly}
\end{equation}
A 6th order accurate central finite difference approximation is derived as follows:
\begin{equation}
	u(x) = \sum_{k=-3}^3 u_{j+k} L_{j+k}(x)
	\label{eq:6order}
\end{equation}
Because only the Lagrange interpolation polynomial depends on $x$ we can find the derivative of $u(x)$ by differentiating $L_{j+k}$ which can be found using the logarithmic differentiation method, resulting in:
\begin{equation}
	\begin{aligned}
		\ln(L_{j+k}(x)) & = \sum_{l=-m, l \neq k}^m \ln\left(\frac{x - x_{j+l}}{x_{j+k} - x_{j+l}}\right)  \\
		                & = \sum_{l=-m, l \neq k}^m \left[\ln(x - x_{j+l}) - \ln(x_{j+k} - x_{j+l})\right]
	\end{aligned}
\end{equation}
Differentiating both sides with respect to $x$
\begin{equation}
	\begin{aligned}
		\frac{1}{L_{j+k}(x)}\frac{d}{dx}L_{j+k}(x) & = \sum_{l=-m, l \neq k}^m \frac{d}{dx}\left[\ln(x - x_{j+l}) - \ln(x_{j+k} - x_{j+l})\right] \\
		                                           & = \sum_{l=-m, l \neq k}^m \frac{d}{dx}\ln(x - x_{j+l})                                       \\
		                                           & = \sum_{l=-m, l \neq k}^m \frac{1}{x - x_{j+l}}
	\end{aligned}
\end{equation}
Solving for the derivative of $L_{j+k}(x)$
\begin{equation}
	\frac{d}{dx}L_{j+k}(x)  = L_{j+k}(x) \sum_{l=-m, l \neq k}^m \frac{1}{x - x_{j+l}}
\end{equation}
Resulting in the derivative of $u(x)$ being:
\begin{equation}
	\begin{aligned}
		\frac{d}{dx}u(x) & = \sum_{k=-3}^3 u_{j+k} \frac{d}{dx}L_{j+k}(x)                                                  \\
		                 & = \sum_{k=-3}^3 u_{j+k} \left[ L_{j+k}(x) \sum_{l=-3, l \neq k}^3 \frac{1}{x - x_{j+l}} \right]
	\end{aligned}
	\label{eq:der_u}
\end{equation}
% 	\begin{aligned}
% 		c_k &= \left. L_{j+k}(x) \sum_{l=-3, l \neq k}^3 \frac{1}{x - x_{j+l}} \right|_{x=x_j}\\
% 		c_k &= \sum_{l=-3, l \neq k}^3 \frac{1}{(j+k-j-l)h} \prod_{m=-3, m \neq k, m \neq l}^3 \frac{j-j-m}{j+k-j-m} \\
% 		c_k &= \frac{1}{h} \sum_{l=-3, l \neq k}^3 \frac{1}{k-l} \prod_{m=-3, m \neq k, m \neq l}^3 \frac{-m}{k-m}\\
% 	\end{aligned}
% \end{equation}
Now if we set $x=x_j$ and plug into \eqref{eq:der_u} we need to examine what happens for different $k$. In order to do so we can rewrite \eqref{eq:der_u} as
\begin{equation}
	\frac{d}{dx}u(x_j) = \sum_{k=-3}^3 u_{j+k} c_k
	\label{eq:c_k}
\end{equation}
For $k=0$ we know that $L_j(x_j) = 1$ by definition of the Lagrange polynomials, resulting in the following coefficient
\begin{equation}
	\begin{aligned}
		c_0 & = \left ( \frac{1}{x_j - x_{j-3}} +  \frac{1}{x_j - x_{j-2}} + \frac{1}{x_j - x_{j-1}} + \frac{1}{x_j - x_{j+1}} + \frac{1}{x_j - x_{j+2}} +\frac{1}{x_j - x_{j+3}} \right) \\
		c_0 & = \left ( \frac{1}{-3\Delta x}  + \frac{1}{-2\Delta x} + \frac{1}{-\Delta x} + \frac{1}{\Delta x} + \frac{1}{2 \Delta x} + \frac{1}{3 \Delta x} \right) = 0
	\end{aligned}
	\label{eq:c_0}
\end{equation}
For the case where $k \neq 0$, the lagrange polynomial is $L_{j+k}(x_j) = 0$, because in the product used for the langrange polynomial will be a factor of $(x_j - x_j) = 0$. However in the product of $L_{j+k}(x) \sum_{l=-3, l \neq k}^3 \frac{1}{x - x_{j+l}} $, we have a division by zero when $l = 0$, this creates the indetermined form $0 \cdot \infty$. \newline
Therefore we compute the limit:
\begin{equation}
	\begin{aligned}
		\lim_{x \rightarrow x_j} c_k & = \lim_{x \rightarrow x_j} \left [ L_{j+k}(x)  \sum_{l=-3, l \neq k}^3 \frac{1}{x - x_{j+l}} \right ]                                                                         \\
		                             & = \lim_{x \rightarrow x_j} \left [ L_{j+k}(x) \left (  \frac{1}{x - x_j} + \sum_{l=-3, l \neq k, l \neq 0}^3 \frac{1}{x - x_{j+l}} \right ) \right ]                          \\
		                             & = \lim_{x \rightarrow x_j} \left [ L_{j+k}(x)  \frac{1}{x - x_j}  + \underbrace{L_{j+k}(x) \sum_{l=-3, l \neq k, l \neq 0}^3 \frac{1}{x - x_{j+l}} }_{\rightarrow 0} \right ] \\
	\end{aligned}
	\label{eq:lim_c_k}
\end{equation}
the second term goes to zero due to $L_{j+k}(x_j) = 0$, but for the first term we can write out the langrange polynomial and take out the term for $l=0$ in the product resulting in
\begin{equation}
	\begin{aligned}
		\lim_{x \rightarrow x_j} c_k & =  \lim_{x \rightarrow x_j} \frac{1}{x - x_j} \frac{x - x_j}{x_{j+k} - x_j} \prod_{l=-3, l \neq k, l \neq 0}^3 \frac{x - x_{j+l}}{x_{j+k} - x_{j+l}} \\
		                             & =  \lim_{x \rightarrow x_j} \frac{1}{x_{j+k} - x_j} \cdot \prod_{l=-3, l \neq k, l \neq 0}^3 \frac{x - x_{j+l}}{x_{j+k} - x_{j+l}}                   \\
		\label{eq:yep}
	\end{aligned}
\end{equation}
Evaluating this at $x = x_j$ leads to a non zero term for $k \neq 0$.
\begin{equation}
	c_k = \frac{1}{x_{j+k} - x_j} \prod_{l=-3, l \neq k, l \neq 0}^3 \frac{x_j - x_{j+l}}{x_{j+k} - x_{j+l}}
	\label{eq:non_zero}
\end{equation}
Using the result from \eqref{eq:c_0} and \eqref{eq:non_zero} leads to the following coefficients:\newline
For $k=-3$:
\begin{equation}
	\begin{aligned}
		c_{-3} & = \frac{1}{x_{j-3} - x_j} \prod_{l=-3, l \neq 0, l \neq -3}^3 \frac{x_j - x_{j+l}}{x_{j-3} - x_{j+l}}                                                                                                                    \\
		       & = \frac{1}{-3\Delta x} \cdot \frac{(x_j - x_{j-2})(x_j - x_{j-1})(x_j - x_{j+1})(x_j - x_{j+2})(x_j - x_{j+3})}{(x_{j-3} - x_{j-2})(x_{j-3} - x_{j-1})(x_{j-3} - x_{j+1})(x_{j-3} - x_{j+2})(x_{j-3} - x_{j+3})} \\
		       & = \frac{1}{-3\Delta x} \cdot \frac{(2\Delta x)(\Delta x)(-\Delta x)(-2\Delta x)(-3\Delta x)}{(-\Delta x)(-2\Delta x)(-4\Delta x)(-5\Delta x)(-6\Delta x)}                                                         \\
		       & = \frac{1}{-3\Delta x} \cdot \frac{-12 \Delta x^5}{-240 \Delta x^5} = \frac{-1}{60\Delta x}                                                                                                                        \\
	\end{aligned}
\end{equation}
For $k=-2$:
\begin{equation}
	\begin{aligned}
		c_{-2} & = \frac{1}{x_{j-2} - x_j} \prod_{l = -3 l \neq 0, l \neq -2}^3 \frac{x_j - x_{j+l}}{x_{j-2} - x_{j+l}}                                                                                                                    \\
		       & = \frac{1}{-2\Delta x} \cdot \frac{(x_j - x_{j-3})(x_j - x_{j-1})(x_j - x_{j+1})(x_j - x_{j+2})(x_j - x_{j+3})}{(x_{j-2} - x_{j-3})(x_{j-2} - x_{j-1})(x_{j-2} - x_{j+1})(x_{j-2} - x_{j+2})(x_{j-2} - x_{j+3})} \\
		       & =  \frac{1}{-2\Delta x} \cdot \frac{(3\Delta x)(\Delta x)(-\Delta x)(-2\Delta x)(-3\Delta x)}{(\Delta x)(-\Delta x)(-3\Delta x)(-4\Delta x)(-5\Delta x)}                                                           \\
		       & = \frac{1}{-2\Delta x} \cdot \frac{-18\Delta x^5}{60 \Delta x^5} = \frac{3}{20\Delta x}
	\end{aligned}
\end{equation}
For $k=-1$:
\begin{equation}
	\begin{aligned}
		c_{-1} & = \frac{1}{x_{j-1} - x_j} \prod_{l=-3, l \neq 0, l \neq -1}^3 \frac{x_j - x_{j+l}}{x_{j-1} - x_{j+l}}                                                                                                                   \\
		       & = \frac{1}{-\Delta x} \cdot \frac{(x_j - x_{j-3})(x_j - x_{j-2})(x_j - x_{j+1})(x_j - x_{j+2})(x_j - x_{j+3})}{(x_{j-1} - x_{j-3})(x_{j-1} - x_{j-2})(x_{j-1} - x_{j+1})(x_{j-1} - x_{j+2})(x_{j-1} - x_{j+3})} \\
		       & = \frac{1}{-\Delta x} \cdot \frac{(3\Delta x)(2\Delta x)(-\Delta x)(-2\Delta x)(-3\Delta x)}{(2\Delta x)(\Delta x)(-2\Delta x)(-3\Delta x)(-4\Delta x)}                                                            \\
		       & = \frac{1}{-\Delta x} \cdot \frac{-36 \Delta x^5}{-48 \Delta x^5} = \frac{-3}{4\Delta x}
	\end{aligned}
\end{equation}
For $k = 0 $ the coefficient was computed in \eqref{eq:c_0} and is $c_0 = 0$\newline
For $k = 1$:
\begin{equation}
	\begin{aligned}
		c_{1} & = \frac{1}{x_{j+1} - x_j} \prod_{l=-3, l \neq 0, l \neq 1}^3 \frac{x_j - x_{j+l}}{x_{j+1} - x_{j+l}}                                                                                                                   \\
		      & = \frac{1}{\Delta x} \cdot \frac{(x_j - x_{j-3})(x_j - x_{j-2})(x_j - x_{j-1})(x_j - x_{j+2})(x_j - x_{j+3})}{(x_{j+1} - x_{j-3})(x_{j+1} - x_{j-2})(x_{j+1} - x_{j-1})(x_{j+1} - x_{j+2})(x_{j+1} - x_{j+3})} \\
		      & = \frac{1}{\Delta x} \cdot \frac{(3\Delta x)(2\Delta x)(\Delta x)(-2\Delta x)(-3\Delta x)}{(4\Delta x)(3\Delta x)(2\Delta x)(-\Delta x)(-2\Delta x)}                                                               \\
		      & =  \frac{1}{\Delta x} \cdot \frac{36 \Delta x^5}{48 \Delta x^5} = \frac{3}{4\Delta x}
	\end{aligned}
\end{equation}
For $k = 2$:
\begin{equation}
	\begin{aligned}
		c_{2} & = \frac{1}{x_{j+2} - x_j} \prod_{l=-3, l \neq 0, l \neq 2}^3 \frac{x_j - x_{j+l}}{x_{j+2} - x_{j+l}}                                                                                                                    \\
		      & = \frac{1}{2\Delta x} \cdot \frac{(x_j - x_{j-3})(x_j - x_{j-2})(x_j - x_{j-1})(x_j - x_{j+1})(x_j - x_{j+3})}{(x_{j+2} - x_{j-3})(x_{j+2} - x_{j-2})(x_{j+2} - x_{j-1})(x_{j+2} - x_{j+1})(x_{j+2} - x_{j+3})} \\
		      & = \frac{1}{2\Delta x} \cdot \frac{(3\Delta x)(2\Delta x)(\Delta x)(-\Delta x)(-3\Delta x)}{(5\Delta x)(4\Delta x)(3\Delta x)(\Delta x)(-\Delta x)}                                                                 \\
		      & = \frac{1}{2\Delta x} \cdot \frac{18 \Delta x^5}{-60 \Delta x^5} = \frac{-3}{20\Delta x}
	\end{aligned}
\end{equation}
For $k = 3$:
\begin{equation}
	\begin{aligned}
		c_{3} & = \frac{1}{x_{j+3} - x_j} \prod_{l=-3, l \neq 0, l \neq 3}^3 \frac{x_j - x_{j+l}}{x_{j+3} - x_{j+l}}                                                                                                                    \\
		      & = \frac{1}{3\Delta x} \cdot \frac{(x_j - x_{j-3})(x_j - x_{j-2})(x_j - x_{j-1})(x_j - x_{j+1})(x_j - x_{j+2})}{(x_{j+3} - x_{j-3})(x_{j+3} - x_{j-2})(x_{j+3} - x_{j-1})(x_{j+3} - x_{j+1})(x_{j+3} - x_{j+2})} \\
		      & = \frac{1}{3\Delta x} \cdot \frac{(3\Delta x)(2\Delta x)(\Delta x)(-\Delta x)(-2\Delta x)}{(6\Delta x)(5\Delta x)(4\Delta x)(2\Delta x)(\Delta x)}                                                                \\
		      & = \frac{1}{3\Delta x} \cdot \frac{12 \Delta x^5}{240 \Delta x^5} = \frac{1}{60\Delta x}
	\end{aligned}
\end{equation}
Finally we can put it all together and 6th order accurate central finite difference approximation is given as:
\begin{equation}
	\begin{aligned}
		\frac{du}{dx} \bigg\vert_{x=x_j} &= u_{j-3} \frac{-1}{60\Delta x} +  u_{j-2} \frac{3}{20\Delta x} + u_{j-1} \frac{-3}{4\Delta x} + u_{j+1} \frac{3}{4\Delta x} + u_{j+2} \frac{-3}{20\Delta x} + u_{j+3}  \frac{1}{60\Delta x}\\
		&= \frac{-u_{j-3} + 9u_{j-2} - 45u_{j-1} + 45u_{j+1} - 9u_{j+2} + u_{j+3} }{60 \Delta x}
	\end{aligned}
	\label{eq:final}
\end{equation}
